user/carol.c
@@ -4,9 +4,9 @@
 
 __attribute__((section(".text.start"))) void _start(void) {
     struct line l = {.n = 0};
-    struct res d = sys(SYS_DERIVE, 1, W | X);
+    struct res d = sys2(SYS_DERIVE, 1, W | X);
     put_s(&l, "carol: asked for write+execute on my data frame, got ");
-    put_rights(&l, sys(SYS_CAPINFO, d.value, 0).value);
+    put_rights(&l, sys1(SYS_CAPINFO, d.x[1]).x[1]);
     put_s(&l, "\n");
     flush(&l);
 
